Implicit generalization duct tape is starting to make sense.

fowl/Offers/OneSorted/IntegerOperations.v
@@ -1,25 +1,38 @@
 From Coq Require Import
   ZArith.ZArith.
 From Maniunfold.Has Require Export
-  OneSorted.BinaryOperation OneSorted.NullaryOperation TwoSorted.LeftAction.
+  TwoSorted.LeftAction.
+From Maniunfold.Is Require Import
+  OneSorted.Group.
 From Maniunfold.Offers Require Export
   OneSorted.PositiveOperations.
 From Maniunfold.ShouldHave Require Import
   OneSorted.AdditiveNotations.
 
+(** TODO Split operation notations. *)
+
+Local Reserved Notation "n '*' x" (at level 40, left associativity).
+Local Reserved Notation "x '^' n" (at level 30, right associativity).
+
+Local Reserved Notation "'_*_'" (at level 0, no associativity).
+Local Reserved Notation "'_^_'" (at level 0, no associativity).
+
+Local Notation "n '*' x" := (positive_op _+_ n x) : positive_scope.
+Local Notation "'_*_'" := (positive_op _+_) (only parsing) : positive_scope.
+
 Section Context.
 
-Context (A : Type) `(HasBinOp A) `(HasNullOp A) `(HasUnOp A).
+Context (A : Type) `{IsGrp A}.
 
 Definition z_op (n : Z) (x : A) : A :=
   match n with
   | Z0 => 0
-  | Zpos p => positive_op _+_ p x
-  | Zneg p => - positive_op _+_ p x
+  | Zpos p => (p * x)%positive
+  | Zneg p => - (p * x)%positive
   end.
-
-Global Arguments z_op !_ _.
 
 Global Instance Z_A_has_l_act : HasLAct Z A := z_op.
 
 End Context.
+
+Arguments z_op {_} _ _ _ !_ _.
