fowl/Offers/OneSorted/NaturalOperations.v
@@ -1,15 +1,28 @@
 From Coq Require Import
   NArith.NArith.
 From Maniunfold.Has Require Export
-  OneSorted.BinaryOperation OneSorted.NullaryOperation TwoSorted.LeftAction.
+  TwoSorted.LeftAction.
+From Maniunfold.Is Require Import
+  OneSorted.Monoid.
 From Maniunfold.Offers Require Export
   OneSorted.PositiveOperations.
 From Maniunfold.ShouldHave Require Import
   OneSorted.AdditiveNotations.
 
+(** TODO Split operation notations. *)
+
+Local Reserved Notation "n '*' x" (at level 40, left associativity).
+Local Reserved Notation "x '^' n" (at level 30, right associativity).
+
+Local Reserved Notation "'_*_'" (at level 0, no associativity).
+Local Reserved Notation "'_^_'" (at level 0, no associativity).
+
+Local Notation "n '*' x" := (positive_op _+_ n x) : positive_scope.
+Local Notation "'_*_'" := (positive_op _+_) (only parsing) : positive_scope.
+
 Section Context.
 
-Context (A : Type) `(HasBinOp A) `(HasNullOp A).
+Context (A : Type) `{IsMon A}.
 
 Fixpoint nat_op (n : nat) (x : A) : A :=
   match n with
@@ -17,18 +30,17 @@ Fixpoint nat_op (n : nat) (x : A) : A :=
   | S p => x + @nat_op p x
   end.
 
-Global Arguments nat_op !_ _.
-
 Global Instance nat_A_has_l_act : HasLAct nat A := nat_op.
 
 Definition n_op (n : N) (x : A) : A :=
   match n with
   | N0 => 0
-  | Npos p => positive_op _+_ p x
+  | Npos p => (p * x)%positive
   end.
 
 Global Instance N_A_has_l_act : HasLAct N A := n_op.
 
-Global Arguments n_op !_ _.
-
 End Context.
+
+Arguments nat_op {_} _ _ !_ _.
+Arguments n_op {_} _ _ !_ _.
