fowl/Offers/OneSorted/Arithmetic.v
@@ -1,25 +1,25 @@
-From Maniunfold.Has Require Export
-  OneSorted.Addition OneSorted.Negation
-  OneSorted.Multiplication OneSorted.Reciprocation.
+From Maniunfold.Has Require Import
+  OneSorted.Reciprocation.
+From Maniunfold.Is Require Import
+  OneSorted.Ring.
 From Maniunfold.ShouldHave Require Import
   OneSorted.ArithmeticNotations.
 
 Section Context.
 
-Context (A : Type) `(HasAdd A) `(HasNeg A).
+(** TODO Use [IsFld] instead. *)
+
+Context (A : Type) `{IsRing A} `(HasRecip A).
 
 (** Subtraction, difference, minus. *)
 
 Definition sub (x y : A) : A := x + (- y).
-
-End Context.
-
-Section Context.
-
-Context (A : Type) `(HasMul A) `(HasRecip A).
 
 (** Division, ratio, obelus. *)
 
 Definition div (x y : A) : A := x * (/ y).
 
 End Context.
+
+Arguments sub {_} _ _ _ _ /.
+Arguments div {_} _ _ _ _ /.
