fowl/Offers/OneSorted/PositiveOperations.v
@@ -1,21 +1,23 @@
 From Coq Require Import
   PArith.PArith.
 From Maniunfold.Has Require Export
-  OneSorted.BinaryOperation TwoSorted.LeftAction.
+  TwoSorted.LeftAction.
+From Maniunfold.Is Require Import
+  OneSorted.Semigroup.
 From Maniunfold.ShouldHave Require Import
   OneSorted.AdditiveNotations.
 
 Section Context.
 
-Context (A : Type) `(HasBinOp A).
+Context (A : Type) `{IsSgrp A}.
 
 Import Pos.
 
 Definition positive_op (n : positive) (x : A) : A :=
   iter_op _+_ n x.
 
-Global Arguments positive_op _ _ /.
-
 Global Instance positive_A_has_l_act : HasLAct positive A := positive_op.
 
 End Context.
+
+Arguments positive_op {_} _ !_ _.
